\documentclass[aspectratio=169]{beamer}
\usepackage{amsmath}
\usepackage[T1]{fontenc}
\usepackage[latin1]{inputenc}
\usepackage{pstricks}
\usepackage{graphicx}
\usefonttheme[onlymath]{serif}

%\usecolortheme{owl}

\begin{document}

\begin{frame}

  \begin{center}
  {\blue $\mathbb{Z}$:} Enteros
  \end{center}

  {\blue $\mathbb{Z}$} es un \textit{anillo conmutativo con $1$}, es decir, tiene {\blue suma} y {\blue producto} tales que:\\


  \begin{center}

    \begin{tabular}{c|c}
      \begin{minipage}{5cm}
        {\blue suma} \\
            \begin{enumerate}
              \item {\blue $(a+b)+c = a+(b+c)$}  para todo $ a,b,c \in \mathbb{Z}$
              \item Existe $0 \in \mathbb{Z}$ tal que {\blue $a+0=0+a=a$}  para todo $a \in \mathbb{Z}$
              \item Si $a \in \mathbb{Z}$, existe $-a \in \mathbb{Z}$ tal que {\blue $a+(-a)= 0$}
              \item {\blue $a+b=b+a$}  para todo $a, b\in \mathbb{Z}$
            \end{enumerate}
      \end{minipage}
      &
      \begin{minipage}{5cm}
            {\blue producto} \\
            \begin{enumerate}
              \item {\blue $(a\cdot b)\cdot c = a\cdot (b\cdot c)$}  para todo $ a,b,c \in \mathbb{Z}$
              \item Existe $1 \in \mathbb{Z}$ tal que {\blue $a\cdot 1=1\cdot a=a$}  para todo $a \in \mathbb{Z}$
              \item {\blue $a\cdot b=b\cdot a$}  para todo $a, b\in \mathbb{Z}$
            \end{enumerate}
      \end{minipage}
    \end{tabular}
  \end{center}

  \begin{center}
  Tambi\'en {\blue $a \cdot (b+c) = a\cdot b + a \cdot c$ } para todo $a, b\in \mathbb{Z}$
  \end{center}
\end{frame}


%%%%%%%%%%%%%%%%%%%%%%%%%%%%%%%%%%%%%%%%%%%%%%%%%%%%%%%%%%%%%%%%%%%%%%%%%%%%%%%%%%%%%%%%%%%%%%%%%%

\begin{frame}
  \begin{center}
    \begin{tabular}{c|c}
      \begin{minipage}{5cm}
        \begin{center}
          {\blue Propiedades} \\
        \end{center}

        \begin{enumerate}
          \item {\blue $a\cdot 0 =0 $}, para todo $a\in \mathbb{Z}$
          \item {\blue $(-1) \cdot a = -a$}, para todo $a\in \mathbb{Z}$
          \item {\blue $a(-b) = -(ab) = (-a)b$}, para todo $a, b\in \mathbb{Z}$
          \item {\blue $(-a)(-b) = ab$}, para todo $a, b\in \mathbb{Z}$
        \end{enumerate}

      \end{minipage}
      &
      \begin{minipage}{5cm}
        \begin{center}
          {\blue Dominio Entero}
        \end{center} \\

        \begin{enumerate}
          \item {\blue $a\cdot b = 0$ } en $\mathbb{Z}$,  implica {\blue $a=0$ o $b=0$} \\
          Equivalente a: \\
          \item {\blue $a\cdot b = a\cdot c, \quad a \neq 0$ }  en $\mathbb{Z}$, implica {\blue $b=c$ }
        \end{enumerate}
      \end{minipage}

    \end{tabular}
  \end{center}
\end{frame}

\end{document}


%%%%%%%%%%%%%%%%%%%%%%%%%%%%%%%%%%%%%%%%%%%%%%%%%%%%%%%%%%%%%%%%%%%%%%%%%%%%%%%%%%%%%%%%%%%%%%%%%%
